examples/Sek/Capacity_proof.v
@@ -3,6 +3,13 @@ From CFML Require Import LibSepGroup WPLibCredits Stdlib.
 Open Scope cf_scope.
 Open Scope record_scope.
 
+From TLC Require Import LibListZ LibMap.
+
+From CFML Require Import LibSepTLCbuffer.
+Import IndexHints.
+
+Require Import ListMisc.
+
 Require Import Capacity_ml.
 
 
@@ -14,6 +21,8 @@ Notation "'K'" := capacity.
 Definition Wrap_up i := If i >= K then i - K else i.
 Definition Wrap_down i := If i < 0 then i + K else i.
 
+Definition IsFull A (c: list A) : Prop :=
+	length c = K.
 
 (* ******************************************************* *)
 (** ** Lemma *)
@@ -21,6 +30,14 @@ Definition Wrap_down i := If i < 0 then i + K else i.
 Lemma capacity_spec :
   capacity > 0.
 Proof. rewrite capacity_cf__; math. Qed.
+
+Lemma NotFull_of_nil : forall A,
+	~ IsFull (@nil A).
+Proof.
+	hint capacity_spec.
+	intros. unfold IsFull. rew_list*.
+Qed.
+
 
 (* ******************************************************* *)
 (** ** Hints *)
@@ -38,11 +55,15 @@ Tactic Notation "unwrap_up" :=
 	unfold Wrap_up; repeat case_if*.
 Tactic Notation "unwrap_up" "in" hyp(H) :=
 	unfold Wrap_up in H; repeat case_if* in H.
+Tactic Notation "unwrap_up" "in" "*" :=
+	unfold Wrap_up in *; repeat case_if*.
 
 Tactic Notation "unwrap_down" :=
 	unfold Wrap_down; repeat case_if*.
 Tactic Notation "unwrap_down" "in" hyp(H) :=
 	unfold Wrap_down in H; repeat case_if* in H.
+Tactic Notation "unwrap_down" "in" "*" :=
+		unfold Wrap_down in *; repeat case_if*.
 
 
 (* ******************************************************* *)
