examples/Sek/PChunkImpl_proof.v
@@ -1,0 +1,341 @@
+Set Implicit Arguments.
+From CFML Require Import LibSepGroup WPLibCredits Stdlib.
+From CFML Require Import WPRecord.
+Open Scope cf_scope.
+Open Scope record_scope.
+(*From CFML Require Import WPDisplay WPRecord.
+Open Scope cf_scope.
+Open Scope record_scope.*)
+
+From TLC Require Import LibListZ LibMap.
+
+From CFML Require Import LibSepTLCbuffer.
+Import IndexHints.
+
+Require Import ListMisc.
+
+Require Import PChunkImpl_ml.
+Require Import PArray_proof.
+Require Import Capacity_proof.
+Require Import EChunkImpl_proof.
+
+
+
+(* Pourquoi je suis obligé de le remettre ?? *)
+Instance MonType_Memory A {IA: Inhab A} {EA: Enc A} :
+	MonType (Memory A) :=	make_MonType (Shared) (Extend).
+
+Ltac xcf_pre tt ::=
+	intros; match goal with |- TripleMon _ _ _ _ => unfold TripleMon | _ => idtac end.
+
+
+(* ******************************************************* *)
+(** ** Representation predicates *)
+
+Record PChunkInv A {IA: Inhab A} (L: list A) (D: list A) (front: int) (size: int) (default: A) : Prop :=
+	mkPChunk_inv {
+		pchunk_in : forall (i: int), 0 <= i < size -> D[Wrap_up (front + i)] = L[i];
+		pchunk_out : forall (i: int), size <= i < K -> D[Wrap_up (front + i)] = default;
+		pchunk_length : length L = size;
+		pchunk_capa : length D = K;
+		pchunk_front : 0 <= front < K;
+		pchunk_size : 0 <= size <= K }.
+
+Definition IsPChunk A {IA: Inhab A} {EA: Enc A} (M: Memory A) (L: list A) (c: pchunk_ A) : Prop :=
+	let (data, front, size, default) := c in
+	exists (D: list A),
+		IsPArray M D data /\
+		PChunkInv L D front size default.
+
+Lemma IsPChunk_inv_IsPArray : forall A (IA: Inhab A) (EA: Enc A) (M: Memory A) (c: pchunk_ A) (L: list A),
+	IsPChunk M L c ->
+	exists D, IsPArray M D (data' c).
+Proof. unfold IsPChunk. intros. destruct c. simpl. destruct~ H as [D [Rdata I]]. Qed.
+
+Lemma IsPChunk_inv_PChunkInv : forall A (IA: Inhab A) (EA: Enc A) (M: Memory A) (c: pchunk_ A) (L: list A),
+	IsPChunk M L c ->
+	exists D, PChunkInv L D (front' c) (size' c) (default' c).
+Proof. unfold IsPChunk. intros. destruct c. simpl. destruct~ H as [D [Rdata I]]. Qed.
+
+Lemma IsPChunk_inv_length : forall A (IA: Inhab A) (EA: Enc A) (M: Memory A) (c: pchunk_ A) (L: list A),
+	IsPChunk M L c -> 0 <= length L <= K.
+Proof.
+	intros. forwards [D I]: IsPChunk_inv_PChunkInv H.
+	forwards~: pchunk_size. forwards~: pchunk_length. 
+Qed.
+
+Hint Resolve IsPChunk_inv_IsPArray IsPChunk_inv_PChunkInv IsPChunk_inv_length.
+
+Definition IsHead A {IA: Inhab A} {EA: Enc A} (M: Memory A) (c: pchunk_ A) : hprop :=
+	IsHead M (data' c).
+
+Definition access_cost A {IA: Inhab A} {EA: Enc A} (ishd: bool) (M: Memory A) (c: pchunk_ A) : hprop :=
+	if ishd then IsHead M c \* \$1 else \$(2 * K + 2).
+
+Lemma access_cost_eq : forall A {IA: Inhab A} {EA: Enc A} (ishd: bool) (M: Memory A) (c: pchunk_ A) (L D: list A),
+	IsPChunk M L c ->
+	IsPArray M D (data' c) ->
+		access_cost ishd M c =
+		parray_rebase_and_get_array_cost ishd M (data' c) D.
+Admitted.
+
+Lemma rebase_cost_true : forall A {IA: Inhab A} {EA: Enc A} (M: Memory A) (pa: PArray_ml.parray_ A) (L: list A),
+	parray_rebase_and_get_array_cost true M pa L = PArray_proof.IsHead M pa \* \$1.
+Admitted.
+
+Lemma rebase_cost_false : forall A {IA: Inhab A} {EA: Enc A} (M: Memory A) (pa: PArray_ml.parray_ A) (L: list A),
+	parray_rebase_and_get_array_cost false M pa L = \$(length L + bound L + 2).
+Admitted.
+
+Hint Resolve access_cost_eq rebase_cost_true.
+
+
+(*************************************************)
+(** Specifications *)
+
+Lemma pchunk_default_spec : forall A (IA: Inhab A) (EA: Enc A) (M: Memory A) (L: list A) (c: pchunk_ A),
+	IsPChunk M L c ->
+	SPEC (pchunk_default c)
+		PRE (\$1)
+		POST \[= default' c].
+Proof. unfolds IsPChunk. introv Rc. xcf. xpay. xvals~. Qed.
+
+Hint Extern 1 (RegisterSpec pchunk_default) => Provide pchunk_default_spec.
+
+Lemma pchunk_create_spec : forall A (IA: Inhab A) (EA: Enc A) (M: Memory A) (a: A),
+	SPEC (pchunk_create a)
+		MONO M
+		PRE (\$(K + 2))
+		POST (fun M' c => \[IsPChunk M' nil c] \* IsHead M' c).
+Proof.
+	xcf. xpay. xapp~ ;=> data M' HM' Rdata.
+	xvals~.
+	unfolds~ IsPChunk. exists (make K a). split~.
+	{ constructors~; intros.
+		{ math. }
+		{ rew_listp~. unwrap_up. }
+		{ rew_listp~. } }
+Qed.
+
+Hint Extern 1 (RegisterSpec pchunk_create) => Provide pchunk_create_spec.
+
+Lemma pchunk_is_empty_spec : forall A (IA: Inhab A) (EA: Enc A) (M: Memory A) (L: list A) (c: pchunk_ A),
+	IsPChunk M L c ->
+	SPEC (pchunk_is_empty c)
+		PRE (\$1)
+		POST (fun b => \[b = isTrue (L = nil)]).
+Proof.
+	introv Rc. xcf~. xpay. xvals~.
+	forwards~ [D I]: IsPChunk_inv_PChunkInv. forwards~ EL: pchunk_length. rewrites <- EL.
+	rewrite* length_zero_eq_eq_nil.
+Qed.
+
+Hint Extern 1 (RegisterSpec pchunk_is_empty) => Provide pchunk_is_empty_spec.
+
+Lemma pchunk_is_full_spec : forall A (IA: Inhab A) (EA: Enc A) (M: Memory A) (L: list A) (c: pchunk_ A),
+	IsPChunk M L c ->
+	SPEC (pchunk_is_full c)
+		PRE (\$1)
+		POST (fun b => \[b = isTrue (IsFull L)]).
+Admitted.
+
+Hint Extern 1 (RegisterSpec pchunk_is_full) => Provide pchunk_is_full_spec.
+
+Lemma pchunk_peek_back_spec : forall A (IA: Inhab A) (EA: Enc A) (ishd: bool) (M: Memory A) (L: list A) (c: pchunk_ A),
+	IsPChunk M L c ->
+	L <> nil ->
+	SPEC (pchunk_peek_back c)
+		PRE (\$5 \* access_cost ishd M c)
+		INV (Shared M)
+		POST (fun x => IsHead M c \* \exists L', \[L = L' & x]).
+Admitted.
+
+Hint Extern 1 (RegisterSpec pchunk_peek_back) => Provide pchunk_peek_back_spec.
+
+Lemma pchunk_pop_back_spec : forall A (IA: Inhab A) (EA: Enc A) (ishd: bool) (M: Memory A) (L: list A) (c: pchunk_ A),
+	IsPChunk M L c ->
+	L <> nil -> 
+	SPEC (pchunk_pop_back c)
+		MONO M
+		PRE (\$11 \* access_cost ishd M c)
+		POST (fun M' '(c', x) => \exists L',
+			IsHead M' c' \*
+			\[IsPChunk M' L' c'] \*
+			\[L = L' & x]).
+Proof.
+	introv Rc HL. xcf. xpay.
+	xapp~ ;=> x L' ->. xlets. xapp.
+	destruct c; simpls. lets~ [D [Rdata [Iin Iout Ilen Icapa Ifront Isz]]]: Rc.
+	unfold IsHead; simpl. xchange~ <- rebase_cost_true D.
+	xapp~ (>> parray_set_spec true M data' D).
+	{ unwrap_up; math. }
+	{	intros pa M' E Rpa. xlets. xvals~.
+		rew_list~ in *.
+		unfold IsPChunk. exists. split~.
+		{ constructors* ;=> i Hi.
+			{ applys_eq* Iin; list_cases*.
+				{ unwrap_up in C; false; math. }
+				{ unwrap_up. } }
+			{ list_cases*.
+				{ applys_eq* Iout. unwrap_up in C. }
+				{ unwrap_up. } } } }
+Qed.
+
+Hint Extern 1 (RegisterSpec pchunk_pop_back) => Provide pchunk_pop_back_spec.
+
+Lemma pchunk_push_back_spec : forall A (IA: Inhab A) (EA: Enc A) (ishd: bool) (M: Memory A) (c: pchunk_ A) (x: A) (L: list A),
+	IsPChunk M L c ->
+	~ (IsFull L) ->
+	SPEC (pchunk_push_back c x)
+		MONO M
+		PRE (\$5 \* access_cost ishd M c)
+		POST (fun M' c' => IsHead M' c' \* \[IsPChunk M' (L & x) c']).
+Proof.
+	introv Rc HL. unfolds IsFull. xcf. simpl. xpay.
+	destruct c; simpls. lets~ [D [Rdata [Iin Iout Ilen Icapa Ifront Isz]]]: Rc.
+	xapp. rewrites~ (>> access_cost_eq L D); simpl. xapp~.
+	{ unwrap_up. }
+	{ intros pa M' E Rpa. xvals~. unfold IsPChunk. exists; split~.
+		{ constructors* ;=> i Hi; list_cases*; unwrap_up in *; false; math. } }
+Qed.
+
+Hint Extern 1 (RegisterSpec pchunk_push_back) => Provide pchunk_push_back_spec.
+
+Lemma pchunk_peek_front_spec : forall A (IA: Inhab A) (EA: Enc A) (ishd: bool) (M: Memory A) (c: pchunk_ A) (L: list A),
+	IsPChunk M L c ->
+	L <> nil ->
+	SPEC (pchunk_peek_front c)
+		PRE (\$5 \* access_cost ishd M c)
+		INV (Shared M)
+		POST (fun x => IsHead M c \* \exists L', \[L = x :: L']).
+Admitted.
+
+Hint Extern 1 (RegisterSpec pchunk_peek_front) => Provide pchunk_peek_front_spec.
+
+Lemma pchunk_pop_front_spec : forall A (IA: Inhab A) (EA: Enc A) (ishd: bool) (M: Memory A) (c: pchunk_ A) (L: list A),
+	IsPChunk M L c ->
+	L <> nil -> 
+	SPEC (pchunk_pop_front c)
+		MONO M
+		PRE (\$11 \* access_cost ishd M c)
+		POST (fun M' '(c', x) => \exists L',
+			IsHead M' c' \*
+			\[IsPChunk M' L' c'] \*
+			\[L = x :: L']).
+Admitted.
+
+Hint Extern 1 (RegisterSpec pchunk_pop_front) => Provide pchunk_pop_front_spec.
+
+Lemma pchunk_push_front_spec : forall A (IA: Inhab A) (EA: Enc A) (ishd: bool) (M: Memory A) (c: pchunk_ A) (x: A) (L: list A),
+	IsPChunk M L c ->
+	~ (IsFull L) ->
+	SPEC (pchunk_push_back c x)
+		MONO M
+		PRE (\$5 \* access_cost ishd M c)
+		POST (fun M' c' => IsHead M' c' \* \[IsPChunk M' (x :: L) c']).
+Admitted.
+
+Hint Extern 1 (RegisterSpec pchunk_push_front) => Provide pchunk_push_front_spec.
+
+Lemma pchunk_get_spec : forall A (IA: Inhab A) (EA: Enc A) (ishd: bool) (M: Memory A) (c: pchunk_ A) (L: list A) (i: int),
+	IsPChunk M L c ->
+	index L i ->
+	SPEC (pchunk_get c i)
+		PRE (\$4 \* access_cost ishd M c)
+		INV (Shared M)
+		POST (fun x => IsHead M c \* \[x = L[i]]).
+Admitted.
+
+Hint Extern 1 (RegisterSpec pchunk_get) => Provide pchunk_get_spec.
+
+Lemma pchunk_set_spec : forall A (IA: Inhab A) (EA: Enc A) (ishd: bool) (M: Memory A) (c: pchunk_ A) (L: list A) (i: int) (x: A),
+	IsPChunk M L c ->
+	index L i ->
+	SPEC (pchunk_set c i x)
+		MONO M
+		PRE (\$5 \* access_cost ishd M c)
+		POST (fun M' c' => IsHead M' c' \* \[IsPChunk M' (L[i := x]) c']).
+Proof.
+	introv Rc Hi. xcf; simpl. xpay. xapp.
+	destruct c; simpls. lets [D [Rdata [Iin Iout Ilen Icapa Ifront Isz]]]: Rc. xchange~ access_cost_eq; simpl. xapp~.
+	{ rew_index in *. unwrap_up. }
+	{ intros pa M' E Rpa. xvals~.
+		unfold IsPChunk. exists; split~.
+		{ constructors* ;=> j Hj; list_cases*; unwrap_up in *; false; math. } }
+Qed.
+
+Hint Extern 1 (RegisterSpec pchunk_set) => Provide pchunk_set_spec.
+
+Lemma pchunk_concat_spec : forall A (IA: Inhab A) (EA: Enc A) (ishd: bool) (M: Memory A) (c0 c1: pchunk_ A) (L0 L1: list A),
+	IsPChunk M L0 c0 ->
+	IsPChunk M L1 c1 ->
+	length L0 + length L1 <= K ->
+	SPEC (pchunk_concat c0 c1)
+		MONO M
+		PRE (if ishd then \$(16 * length L1) \* IsHead M c0 \* IsHead M c1)
+		POST (fun M' c' => \[IsPChunk M' (L0 ++ L1) c']).
+Proof.
+	introv Rc0 Rc1 Hlen. gen c0 L0 c1. induction_wf IH: list_sub L1.
+	introv Rc0 Hlen; introv Rc1. xcf; simpl. xpay.
+	xapp~. xif ;=> C.
+	(* TODO: update specs for PArray, operations on pa which extend M MUST preserve IsHead predicates for all pa' <> pa
+	Else bad complexity analysis *)
+	skip.
+Qed.
+
+(* If one is empty, we do not get heads necessarily (but always constant time).
+Function parray_touch which rebases (thus giving IsHead predicate), which we call
+in the base case to ensure that we always return a head version ? *)
+
+Hint Extern 1 (RegisterSpec pchunk_concat) => Provide pchunk_concat_spec.
+
+Lemma pchunk_displace_spec : forall A (IA: Inhab A) (EA: Enc A) (M: Memory A) (c0 c1: pchunk_ A) (L0 L1: list A) (k: int),
+	IsPChunk M L0 c0 ->
+	IsPChunk M L1 c1 ->
+	0 <= k <= length L0 ->
+	length L1 + k <= K ->
+	SPEC (pchunk_displace c0 c1 k)
+		MONO M
+		PRE (\$(2 * K + 2 + k))
+		POST (fun M' '(c0', c1') =>
+			(If k > 0 then IsHead M' c0 \* IsHead M' c1 else \[]) \*
+			\exists L0' L1',
+			\[L0 = L0' ++ L1'] \*
+			\[length L1' = k] \*
+			\[IsPChunk M' L0' c0'] \*
+			\[IsPChunk M' (L1' ++ L1) c1']).
+Admitted.
+
+Hint Extern 1 (RegisterSpec pchunk_displace) => Provide pchunk_displace_spec.
+
+Lemma pchunk_split_spec : forall A (IA: Inhab A) (EA: Enc A) (M: Memory A) (c: pchunk_ A) (L: list A) (k: int),
+	IsPChunk M L c ->
+	0 <= k <= length L ->
+	SPEC (pchunk_split c k)
+		MONO M
+		PRE \[]
+		POST (fun M' '(c0, c1) =>
+			IsHead M' c1 \*
+			(If k <> length L then IsHead M' c0 else \[]) \*
+			\exists L0 L1,
+			\[L0 = L0 ++ L1] \*
+			\[length L0 = k] \*
+			\[IsPChunk M' L0 c0] \*
+			\[IsPChunk M' L1 c1]).
+Admitted.
+
+Hint Extern 1 (RegisterSpec pchunk_displace) => Provide pchunk_displace_spec.
+
+Lemma pchunk_of_echunk_spec : forall A (IA: Inhab A) (EA: Enc A) (M: Memory A) (ec: EChunkImpl_ml.echunk_ A) (L: list A),
+	SPEC (pchunk_of_echunk ec)
+		MONO M
+		PRE (\$3 \* ec ~> EChunk L)
+		POST (fun M' pc => IsHead M' pc \* \[IsPChunk M' L pc]).
+Proof.
+	xcf*. xpay. xapp ;=> [[[data front] size] default]. xpull ;=> D I. xmatch.
+	xapp ;=> pa M' E Rpa. xvals~.
+	unfold IsPChunk. exists D. split~.
+	destruct I. constructors~.
+Qed.
+
+Hint Extern 1 (RegisterSpec pchunk_of_echunk) => Provide pchunk_of_echunk_spec.
